\documentclass{beamer}
\usetheme{CambridgeUS}
\usepackage{enumerate}
\usepackage{amsmath,amsfonts,amssymb}
\usepackage{setspace}
\usepackage{float}
\usepackage{cellspace}
\usepackage{longtable}
\newcounter{saveenumerate}
\newcommand{\saveenumerate}{\setcounter{saveenumerate}{\value{enumi}}}
\newcommand{\restartenumerate}{\setcounter{enumi}{\value{saveenumerate}}}
\title{Assignment 5} 
\author{Harshit Pant\\CS21BTECH11021}
\date{}
\providecommand{\pr}[1]{\ensuremath{\Pr\left(#1\right)}}
%\logo{\large \LaTeX{}}
\begin{document}
\begin{frame}
    \titlepage 
\end{frame}
\begin{frame}{Outline}
    %\tableofcontents
\begin{abstract}
This document contains the solution to Exercise 13.2 Question 11 of Chapter 13 (Probability) in the NCERT Class 12 Exemplar.
\end{abstract}
\textbf{Ex 13.2 Q)11: }Given two independent events A and B such that $\pr{A}=0.3$, $\pr{B}=0.6$. Find
\begin{enumerate}[i]
\item $\pr{AB}$
\item $\pr{AB'}$
\item $\pr{A+B}$
\item $\pr{A'B'}$
\end{enumerate}
\end{frame}

\begin{frame}
\textbf{Solution:} 
\begin{enumerate}[i]
\item Since A and B are independent events.
		\begin{align}
		\pr{AB}&=\pr{A}\times\pr{B}\\
			\pr{AB}&=0.3\times0.6\\
			\pr{AB}&=0.18
			\end{align}
			%\end{enumerate}
			%\end{frame}
\item  %Since B is an independent event $\therefore\,B'$ is also an independent event.
			\begin{align}
			A&=A(B+B')\\
			A&=AB+AB'
			\end{align}
			Since $AB$ and $AB'$ are mutually exclusive events $\therefore$
			\begin{align}
			\pr{A}&=\pr{AB}+\pr{AB'}\\
			\pr{AB'}&=\pr{A}-\pr{AB}\\
			\pr{AB'}&=0.3-0.18\\
			\pr{AB'}&=0.12
			\end{align}
			\saveenumerate
			\end{enumerate}
			\end{frame}
			\begin{frame}
			\begin{enumerate}[i]
			\restartenumerate
\item  \begin{align}
			AB'+B&=(B+B')(B+A)\\
			AB'+B&=B+A\\
			\pr{A+B}&=\pr{AB'+B}
			\end{align}
			Since $AB'$ and $B$ are mutually exclusive events $\therefore$
			\begin{align}
			\pr{A+B}&=\pr{AB'}+\pr{B}
			\end{align}
			Substituting $\pr{AB'}$,
			\begin{align}
			\pr{A+B}&=\pr{B}+\pr{A}-\pr{AB}\\
			\pr{A+B}&=0.3+0.6-0.18\\
			\pr{A+ B}&=0.72
			\end{align}
			\saveenumerate
			\end{enumerate}
			\end{frame}
			\begin{frame}
			\begin{enumerate}[i]
			\restartenumerate
\item  By De-Morgan's Principle-
			\begin{align}
			\pr{A'B'}&=\pr{(A+B)'}\\
			\pr{A'B'}&=1-0.72\\
			\pr{A'B'}&=0.28
			\end{align}		
\end{enumerate}
\end{frame}
\end{document}